better treatement of type inv

theories/BasicMetaTheory.v
@@ -1090,144 +1090,80 @@ Qed.
 (* newer versions of inversion lemmas.
    TODO: replace in Confluence.v the occurrences of older inversion lemmas by the newer ones *)
 
-Lemma type_inv_var' Γ l x T :
-  Γ ⊢< l > var x : T →
-  ∃ A, Γ ∋< l > x : A ∧ Γ ⊢< Ax l > T ≡ A : Sort l.
+
+Definition type_inv_statement Γ l t T :=
+  match t with 
+  | var x => 
+    ∃ A, Γ ∋< l > x : A ∧ Γ ⊢< Ax l > T ≡ A : Sort l
+  | Sort i => 
+    l = Ax (Ax i) /\
+    Γ ⊢< Ax (Ax (Ax i)) > T ≡ Sort (Ax i) : Sort (Ax (Ax i))
+  | Pi i j A B =>
+    Γ ⊢< Ax i > A : Sort i /\
+    Γ ,, (i, A) ⊢< Ax j > B : Sort j /\
+    l = Ax (Ru i j) /\
+    Γ ⊢< Ax (Ax (Ru i j)) > T ≡ Sort (Ru i j) : Sort (Ax (Ru i j))
+  | lam i j A B t =>
+    Γ ⊢< Ax i > A : Sort i /\
+    Γ ,, (i , A) ⊢< Ax j > B : Sort j /\
+    Γ ,, (i , A) ⊢< j > t : B /\
+    l = Ru i j /\
+    Γ ⊢< Ax (Ru i j) > T ≡ Pi i j A B : Sort (Ru i j)
+  | app i j A B t u =>
+    Γ ⊢< Ax i > A : Sort i /\
+    Γ ,, (i , A) ⊢< Ax j > B : Sort j /\
+    Γ ⊢< Ru i j > t : Pi i j A B /\
+    Γ ⊢< i > u : A /\
+    l = j /\
+    Γ ⊢< Ax j > T ≡ B <[ u.. ] : Sort j
+  | Nat =>
+    l = ty 1 /\
+    Γ ⊢< ty 2 > T ≡ Sort (ty 0) : Sort (ty 1)
+  | zero =>
+    l = ty 0 /\
+    Γ ⊢< ty 1 > T ≡ Nat : Sort (ty 0)
+  | succ t =>
+    Γ ⊢< ty 0 > t : Nat /\
+    l = ty 0 /\
+    Γ ⊢< ty 1 > T ≡ Nat : Sort (ty 0)
+  | rec i P p_zero p_succ t =>
+    Γ ,, (ty 0 , Nat) ⊢< Ax i > P : Sort i /\
+    Γ ⊢< i > p_zero : P <[ zero .. ] /\
+    Γ ,, (ty 0 , Nat) ,, (i , P) ⊢< i > p_succ : P <[ (succ (var 1)) .: (shift >> (shift >> var)) ] /\
+    Γ ⊢< ty 0 > t : Nat /\
+    l = i /\
+    Γ ⊢< Ax i > T ≡ P <[ t.. ] : Sort i
+  | box => 
+    False
+  end.
+
+
+Lemma type_inv Γ l t T : 
+  Γ ⊢< l > t : T -> 
+  type_inv_statement Γ l t T.
 Proof.
-  intro H.
+  intros.
   apply validity_ty_ty in H as T_Wt.
-  dependent induction H.
-  - eexists. split; eauto using conv_refl.
-  - edestruct IHtyping as (C & eq & A_eq_C); eauto using validity_conv_left. eexists. split; eauto using conv_trans, conv_sym.
-Qed.
-
-Lemma type_inv_sort' Γ l' i T:
-  Γ ⊢< l' > Sort i : T ->
-  l' = Ax (Ax i) /\
-  Γ ⊢< Ax (Ax (Ax i)) > T ≡ Sort (Ax i) : Sort (Ax (Ax i)).
-Proof.
-  intro H.
-  apply validity_ty_ty in H as T_Wt.
-  dependent induction H.
-  - repeat split; eauto using conv_refl.
-  - edestruct IHtyping as (l_eq & conv); eauto using validity_conv_left.
-    rewrite l_eq in *. repeat split; eauto using conv_trans, conv_sym.
-Qed.
-
-Lemma type_inv_pi' Γ l' i j A B T:
-  Γ ⊢< l' > Pi i j A B : T ->
-  Γ ⊢< Ax i > A : Sort i /\
-  Γ ,, (i, A) ⊢< Ax j > B : Sort j /\
-  l' = Ax (Ru i j) /\
-  Γ ⊢< Ax (Ax (Ru i j)) > T ≡ Sort (Ru i j) : Sort (Ax (Ru i j)).
-Proof.
-  intro H.
-  apply validity_ty_ty in H as T_Wt.
-  dependent induction H.
-  - repeat split; eauto using conv_refl.
-  - edestruct IHtyping as (AWt & BWt & l_eq & conv); eauto using validity_conv_left.
-    rewrite l_eq in *. repeat split; eauto using conv_trans, conv_sym.
-Qed.
-
-Lemma type_inv_lam' Γ i j A B t T l :
-      Γ ⊢< l > lam i j A B t : T ->
-      Γ ⊢< Ax i > A : Sort i /\
-      Γ ,, (i , A) ⊢< Ax j > B : Sort j /\
-      Γ ,, (i , A) ⊢< j > t : B /\
-      l = Ru i j /\
-      Γ ⊢< Ax (Ru i j) > T ≡ Pi i j A B : Sort (Ru i j).
-Proof.
-  intro H.
-  apply validity_ty_ty in H as T_Wt.
-  dependent induction H; eauto.
-  - repeat split; eauto using conv_refl.
-  - edestruct IHtyping as (AWt & BWt & tWt & l_eq & conv); eauto using validity_conv_left.
-    rewrite l_eq in *. repeat split; eauto using conv_trans, conv_sym.
-Qed.
-
-Lemma type_inv_app' Γ i j A B t u l T :
-      Γ ⊢< l > app i j A B t u : T ->
-      Γ ⊢< Ax i > A : Sort i /\
-      Γ ,, (i , A) ⊢< Ax j > B : Sort j /\
-      Γ ⊢< Ru i j > t : Pi i j A B /\
-      Γ ⊢< i > u : A /\
-      l = j /\
-      Γ ⊢< Ax j > T ≡ B <[ u.. ] : Sort j.
-Proof.
-  intro H.
-  apply validity_ty_ty in H as T_Wt.
-  dependent induction H; eauto.
-  - repeat split; eauto using conv_refl.
-  - edestruct IHtyping as (AWt & BWt & tWt & uWt & l_eq & conv); eauto using validity_conv_left.
-    rewrite l_eq in *. repeat split; eauto using conv_trans, conv_sym.
-Qed.
-
-Lemma type_inv_nat' Γ l' T:
-  Γ ⊢< l' > Nat : T ->
-  l' = ty 1 /\
-  Γ ⊢< ty 2 > T ≡ Sort (ty 0) : Sort (ty 1).
-Proof.
-  intro H.
-  apply validity_ty_ty in H as T_Wt.
-  dependent induction H.
-  - repeat split; eauto using conv_refl.
-  - edestruct IHtyping as (l_eq & conv); eauto using validity_conv_left.
-    rewrite l_eq in *. repeat split; eauto using conv_trans, conv_sym.
-Qed.
-
-
-Lemma type_inv_zero' Γ l' T:
-  Γ ⊢< l' > zero : T ->
-  l' = ty 0 /\
-  Γ ⊢< ty 1 > T ≡ Nat : Sort (ty 0).
-Proof.
-  intro H.
-  apply validity_ty_ty in H as T_Wt.
-  dependent induction H.
-  - repeat split; eauto using conv_refl.
-  - edestruct IHtyping as (l_eq & conv); eauto using validity_conv_left.
-    rewrite l_eq in *. repeat split; eauto using conv_trans, conv_sym.
-Qed.
-
-
-Lemma type_inv_succ' Γ t T l :
-      Γ ⊢< l > succ t : T ->
-      Γ ⊢< ty 0 > t : Nat /\
-      l = ty 0 /\
-      Γ ⊢< ty 1 > T ≡ Nat : Sort (ty 0).
-Proof.
-  intro H.
-  apply validity_ty_ty in H as T_Wt.
-  dependent induction H; eauto.
-  - repeat split; eauto using conv_refl.
-  - edestruct IHtyping as (tWt & l_eq & conv); eauto using validity_conv_left.
-    rewrite l_eq in *. repeat split; eauto using conv_trans, conv_sym.
-Qed.
-
-Lemma type_inv_rec' Γ l' l P p_zero p_succ t T :
-  Γ ⊢< l' > rec l P p_zero p_succ t : T ->
-  Γ ,, (ty 0 , Nat) ⊢< Ax l > P : Sort l /\
-  Γ ⊢< l > p_zero : P <[ zero .. ] /\
-  Γ ,, (ty 0 , Nat) ,, (l , P) ⊢< l > p_succ : P <[ (succ (var 1)) .: (shift >> (shift >> var)) ] /\
-  Γ ⊢< ty 0 > t : Nat /\
-  l' = l /\
-  Γ ⊢< Ax l > T ≡ P <[ t.. ] : Sort l.
-Proof.
-  intro H.
-  apply validity_ty_ty in H as T_Wt.
-  dependent induction H; eauto.
-  - repeat split; eauto using conv_refl.
-  - edestruct IHtyping as (PWt & p_zeroWt & p_succWt & tWt & l_eq & conv); eauto using validity_conv_left.
-    rewrite l_eq in *. repeat split; eauto using conv_trans, conv_sym.
-Qed.
-
-
-Lemma type_inv_box' Γ T l :
-      Γ ⊢< l > box : T ->
-      False.
-Proof.
-  intro H.
-  dependent induction H; eauto.
+  destruct t; simpl; dependent induction H; eauto 7 using conv_refl.
+  - edestruct IHtyping as (C & eq & A_eq_C); 
+      eauto using validity_conv_left, conv_trans, conv_sym.
+  - edestruct IHtyping as (l_eq & conv); 
+      try rewrite l_eq in *; eauto using validity_conv_left, conv_trans, conv_sym.
+  - edestruct IHtyping as (AWt & BWt & l_eq & conv); 
+      try rewrite l_eq in *; eauto 9 using validity_conv_left, conv_trans, conv_sym.
+  - edestruct IHtyping as (AWt & BWt & tWt & l_eq & conv); 
+      try rewrite l_eq in *; eauto 9 using validity_conv_left, conv_trans, conv_sym.
+  - edestruct IHtyping as (AWt & BWt & tWt & uWt & l_eq & conv); 
+      try rewrite l_eq in *; eauto 9 using validity_conv_left, conv_trans, conv_sym.
+  - edestruct IHtyping as (l_eq & conv); 
+      try rewrite l_eq in *; eauto 9 using validity_conv_left, conv_trans, conv_sym.
+  - edestruct IHtyping as (l_eq & conv); 
+      try rewrite l_eq in *; eauto 9 using validity_conv_left, conv_trans, conv_sym.
+  - edestruct IHtyping as (tWt & l_eq & conv); 
+      try rewrite l_eq in *; eauto 9 using validity_conv_left, conv_trans, conv_sym.
+  - edestruct IHtyping as (PWt & p_zeroWt & p_succWt & tWt & l_eq & conv); 
+      try rewrite l_eq in *; eauto 9 using validity_conv_left, conv_trans, conv_sym.
+  - edestruct IHtyping; eauto using validity_conv_left.
 Qed.
 
 Theorem var_unicity Γ l x A l' A' : 
@@ -1247,22 +1183,22 @@ Theorem type_sort_unicity : forall Γ l l' t A B, Γ ⊢< l > t : A ->  Γ ⊢< 
 Proof.
   intros.
   induction H.
-  - eapply type_inv_var' in H0 as (A' & H1' & Hconv).
+  - eapply type_inv in H0 as (A' & H1' & Hconv).
     eapply var_unicity in H1 as (HA & HB); eauto. subst. eauto using conv_sym.
-  - eapply type_inv_sort' in H0 as (HA & HB ). subst. eauto using conv_sym.
-  - eapply type_inv_pi' in H0 as (_ & _ & eq & conv).
+  - eapply type_inv in H0 as (HA & HB ). subst. eauto using conv_sym.
+  - eapply type_inv in H0 as (_ & _ & eq & conv).
     subst. eauto using conv_sym.
-  - eapply type_inv_lam' in H0 as (_ & _ & _ & eq & conv).
+  - eapply type_inv in H0 as (_ & _ & _ & eq & conv).
     subst. eauto using conv_sym.
-  - eapply type_inv_app' in H0 as (_ & _ & _ & _ & eq & conv).
+  - eapply type_inv in H0 as (_ & _ & _ & _ & eq & conv).
     subst. eauto using conv_sym.
-  - eapply type_inv_nat' in H0 as (eq & conv). 
+  - eapply type_inv in H0 as (eq & conv). 
     subst. eauto using conv_sym.
-  - eapply type_inv_zero' in H0 as (eq & conv). 
+  - eapply type_inv in H0 as (eq & conv). 
     subst. eauto using conv_sym.
-  - eapply type_inv_succ' in H0 as (_ & eq & conv). 
+  - eapply type_inv in H0 as (_ & eq & conv). 
     subst. eauto using conv_sym.
-  - eapply type_inv_rec' in H0 as (_ & _ & _ & _ & eq & conv). 
+  - eapply type_inv in H0 as (_ & _ & _ & _ & eq & conv). 
     subst. eauto using conv_sym.
   - eapply IHtyping in H0 as (HA & HB). eauto using conv_sym, conv_trans.
 Qed.
@@ -1289,7 +1225,7 @@ Proof.
   intros hx hctx.
   eapply type_var in hx; eauto using validity_ctx_conv_left.
   eapply conv_in_ctx_ty in hx; eauto.
-  eapply type_inv_var' in hx as 
+  eapply type_inv in hx as 
     (A0 & varin & conv).
   exists A0. split; eauto.
   eauto using conv_in_ctx_conv, ctx_conv_sym.
